src/cbor/pulse/raw/CBOR.Pulse.Raw.Nondet.Common.fsti
@@ -14,21 +14,7 @@ val cbor_nondet_t: Type0
 val cbor_nondet_match: perm -> cbor_nondet_t -> Spec.cbor -> slprop
 
 inline_for_extraction noextract [@@noextract_to "krml"]
-val cbor_nondet_reset_perm
-  (p: perm)
-  (c: cbor_nondet_t)
-  (r: Ghost.erased Spec.cbor)
-  (q: perm)
-: stt cbor_nondet_t
-  (requires
-    cbor_nondet_match p c r
-  )
-  (ensures fun c' ->
-    cbor_nondet_match q c' r **
-    Trade.trade
-      (cbor_nondet_match q c' r)
-      (cbor_nondet_match p c r)
-  )
+val cbor_nondet_reset_perm (_: unit) : reset_perm_t #_ cbor_nondet_match
 
 val cbor_nondet_share
   (_: unit)
@@ -38,111 +24,9 @@ val cbor_nondet_gather
   (_: unit)
 : CBOR.Pulse.API.Base.gather_t u#0 u#0 #_ #_ cbor_nondet_match
 
-noextract [@@noextract_to "krml"]
-let cbor_nondet_validate_post
-  (map_key_bound: option SZ.t)
-  (strict_check: bool)
-  (v: Seq.seq U8.t)
-  (res: SZ.t)
-: Tot prop
-=
-  let r = Spec.cbor_parse v in
-  if SZ.v res = 0
-  then (Some? r ==> (Some? map_key_bound /\ Spec.cbor_map_key_depth (fst (Some?.v r)) > SZ.v (Some?.v map_key_bound)))
-  else (
-    Some? r /\
-    SZ.v res == snd (Some?.v r) /\
-    ((Some? map_key_bound /\ strict_check) ==> Spec.cbor_map_key_depth (fst (Some?.v r)) <= SZ.v (Some?.v map_key_bound))
-  )
-
-inline_for_extraction
-noextract [@@noextract_to "krml"]
-let cbor_nondet_validate_t
-=
-  (map_key_bound: option SZ.t) ->
-  (strict_check: bool) ->
-  (input: S.slice U8.t) ->
-  (#pm: perm) ->
-  (#v: Ghost.erased (Seq.seq U8.t)) ->
-  stt SZ.t
-    (pts_to input #pm v)
-    (fun res -> pts_to input #pm v ** pure (
-      cbor_nondet_validate_post map_key_bound strict_check v res
-    ))
-
 val cbor_nondet_validate (_: unit) : cbor_nondet_validate_t
 
-noextract [@@noextract_to "krml"]
-let cbor_nondet_parse_valid_post
-  (v: Seq.seq U8.t)
-  (v': Spec.cbor)
-: Tot prop
-= let w = Spec.cbor_parse v in
-  Some? w /\
-  v' == fst (Some?.v w)
-
-inline_for_extraction
-noextract [@@noextract_to "krml"]
-let cbor_nondet_parse_valid_t
-  (#cbor_nondet_t: Type)
-  (cbor_nondet_match: perm -> cbor_nondet_t -> Spec.cbor -> slprop)
-=
-  (input: S.slice U8.t) ->
-  (len: SZ.t) ->
-  (#pm: perm) ->
-  (#v: Ghost.erased (Seq.seq U8.t)) ->
-  stt cbor_nondet_t
-    (pts_to input #pm v ** pure (
-      cbor_nondet_validate_post None false v len /\
-      SZ.v len > 0
-    ))
-    (fun res -> exists* p' v' .
-      cbor_nondet_match p' res v' **
-      Trade.trade (cbor_nondet_match p' res v') (pts_to input #pm v) ** pure (
-        cbor_nondet_parse_valid_post v v'
-    ))
-
 val cbor_nondet_parse_valid (_: unit) : cbor_nondet_parse_valid_t #cbor_nondet_t cbor_nondet_match
-
-noextract [@@noextract_to "krml"]
-let cbor_nondet_serialize_postcond
-  (y: Spec.cbor)
-  (v: Seq.seq U8.t)
-  (v': Seq.seq U8.t)
-  (res: option SZ.t)
-: Tot prop
-= match res with
-  | None -> True // TODO: specify maximum length
-  | Some len ->
-    SZ.v len <= Seq.length v' /\
-    Seq.length v' == Seq.length v /\
-    Seq.equal (Seq.slice v' (SZ.v len) (Seq.length v)) (Seq.slice v (SZ.v len) (Seq.length v)) /\
-    Spec.cbor_parse v' == Some (y, SZ.v len)
-
-noextract [@@noextract_to "krml"]
-let cbor_nondet_serialize_postcond_c
-  (y: Spec.cbor)
-  (v: Seq.seq U8.t)
-  (v': Seq.seq U8.t)
-  (res: SZ.t)
-: Tot prop
-= cbor_nondet_serialize_postcond y v v' (if res = 0sz then None else Some res)
-
-inline_for_extraction
-let cbor_nondet_serialize_t
-  (#cbordet: Type)
-  (cbor_det_match: perm -> cbordet -> Spec.cbor -> slprop)
-=
-  (x: cbordet) ->
-  (output: S.slice U8.t) ->
-  (#y: Ghost.erased Spec.cbor) ->
-  (#pm: perm) ->
-  (#v: Ghost.erased (Seq.seq U8.t)) ->
-  stt (option SZ.t)
-    (cbor_det_match pm x y ** pts_to output v)
-    (fun res -> exists* v' . cbor_det_match pm x y ** pts_to output v' ** pure (
-      cbor_nondet_serialize_postcond y v v' res
-    ))
 
 val cbor_nondet_serialize
   (_: unit)
@@ -256,6 +140,8 @@ val cbor_nondet_mk_string (_: unit) : mk_string_t u#0 #_ cbor_nondet_match
 val cbor_nondet_mk_tagged (_: unit) : mk_tagged_t #_ cbor_nondet_match
 
 val cbor_nondet_mk_array (_: unit) : mk_array_t #_ cbor_nondet_match
+
+val cbor_nondet_mk_map_entry (_: unit) : mk_map_entry_t #_ #_ cbor_nondet_match cbor_nondet_map_entry_match
 
 val cbor_nondet_mk_map_gen (_: unit)
 : mk_map_gen_by_ref_t #cbor_nondet_t #cbor_nondet_map_entry_t cbor_nondet_match cbor_nondet_map_entry_match
